src/ListLemmas.v
@@ -1113,7 +1113,19 @@ intros0 HP Hxy. inv_using distinct_app_inv' Hxy.
 eapply HP; eauto using distinct_disjoint.
 Qed.
 
-Lemma disjoint_dec {A}
+Definition distinct_dec {A}
+    (A_eq_dec : forall (x y : A), { x = y } + { x <> y })
+    (xs : list A) : { distinct xs } + { ~ distinct xs }.
+induction xs.
+- left. constructor.
+- rename a into x.
+  destruct (in_dec A_eq_dec x xs).
+    { right. inversion 1. auto. }
+  destruct IHxs; [ | right; inversion 1; eauto ].
+  left. constructor; eauto.
+Defined.
+
+Definition disjoint_dec {A}
     (A_eq_dec : forall (x y : A), { x = y } + { x <> y })
     (xs ys : list A) : { disjoint xs ys } + { ~ disjoint xs ys }.
 induction xs.
@@ -1123,7 +1135,7 @@ induction xs.
     { right. inversion 1. on >Forall, invc. auto. }
   destruct IHxs; [ | right; inversion 1; eauto ].
   left. on >@disjoint, invc. constructor; eauto.
-Qed.
+Defined.
   
 
 
